better proof of independence with respect to the dynamic values in the environment

asm.v
@@ -84,42 +84,42 @@ Fixpoint exec_asm
 Fixpoint env_to_mem (l : list (string * Z)) : list Z :=
   match l with (s, v) :: l' => v :: env_to_mem l' | nil => nil end.
 
-Fixpoint symbol_index (l : list (string * Z))(s : string) : nat :=
+Fixpoint symbol_index (l : list string)(s : string) : nat :=
   match l with
   | nil => 0
-  | (s', _) :: l' =>
+  | s' :: l' =>
     if string_dec s s' then 0 else S (symbol_index l' s)
   end.
 
-Fixpoint compile_aexp (env : list (string * Z))
+Fixpoint compile_aexp (symbols : list string)
   (e : aexpr0 string) : list assembly :=
   match e with
-  | avar s => [load (symbol_index env s)]
+  | avar s => [load (symbol_index symbols s)]
   | anum n => [push n]
   | aplus e1 e2 =>
-    compile_aexp env e1 ++ compile_aexp env e2 ++ [add]
+    compile_aexp symbols e1 ++ compile_aexp symbols e2 ++ [add]
   end.
 
-Definition compile_bexp (env : list (string * Z))
+Definition compile_bexp (symbols : list string)
   (b : bexpr0 string) : list assembly :=
   match b with
   | blt e1 e2 => 
-    compile_aexp env e1 ++ compile_aexp env e2 ++ [cmp]
+    compile_aexp symbols e1 ++ compile_aexp symbols e2 ++ [cmp]
   end.
 
-Fixpoint compile_instr (env : list (string * Z))(loc : nat)
+Fixpoint compile_instr (symbols : list string)(loc : nat)
   (i : instr0 string) {struct i} : list assembly :=
 match i with
 | assign s e =>
-  let cp_exp := compile_aexp env e in
-  compile_aexp env e ++ [store (symbol_index env s)]
+  let cp_exp := compile_aexp symbols e in
+  compile_aexp symbols e ++ [store (symbol_index symbols s)]
 | sequence i1 i2 =>
-  let pg1 := compile_instr env loc i1 in
-  let pg2 := compile_instr env (loc + length pg1) i2 in
+  let pg1 := compile_instr symbols loc i1 in
+  let pg2 := compile_instr symbols (loc + length pg1) i2 in
   pg1 ++ pg2
 | while b i1 =>
-  let pge := compile_bexp env b in
-  let pgi := compile_instr env (loc + length pge + 1) i1 in
+  let pge := compile_bexp symbols b in
+  let pgi := compile_instr symbols (loc + length pge + 1) i1 in
   pge ++ branch (loc + length pge + length pgi + 2) ::
   pgi ++ [goto loc]
 | skip => []
@@ -137,7 +137,8 @@ Import dyn.
 
 Lemma exec_avar : forall n env e v pg1 pg2 stk,
   aeval env e v -> e = avar n ->
-   exec_asm 1 (pg1 ++ compile_aexp env e ++ pg2) stk (env_to_mem env)
+   exec_asm 1 (pg1 ++ compile_aexp
+                        (map fst env) e ++ pg2) stk (env_to_mem env)
    (length pg1) =
    (v :: stk, env_to_mem env, (length pg1 + 1)%nat).
 Proof.
@@ -183,10 +184,10 @@ Lemma exec_aexp :
   forall env e v pg1 pg2 stk,
   aeval env e v ->
   exists ec, 
-  exec_asm ec (pg1 ++ compile_aexp env e ++ pg2)
+  exec_asm ec (pg1 ++ compile_aexp (map fst env) e ++ pg2)
        stk (env_to_mem env) (length pg1) =
   (v :: stk, env_to_mem env,
-   (length pg1 + length (compile_aexp env e))%nat).
+   (length pg1 + length (compile_aexp (map fst env) e))%nat).
 Proof.
 intros env e v pg1 pg2 stk dyn; revert pg1 pg2 stk.
 induction dyn as [r n | r x v | r x y v v' xny dyn Ih| 
@@ -202,9 +203,10 @@ induction dyn as [r n | r x v | r x y v v' xny dyn Ih|
     now constructor.
   easy.
 intros pg1 pg2 stk.
-destruct (Ih1 pg1 (compile_aexp r e2 ++ [add] ++ pg2) stk) as [ec1 Pec1].
-destruct (Ih2 (pg1 ++ (compile_aexp r e1)) (add :: pg2) (v1 :: stk)) as
-   [ec2 Pec2].
+destruct (Ih1 pg1 (compile_aexp (map fst r) e2 ++ [add] ++ pg2) stk)
+   as [ec1 Pec1].
+destruct (Ih2 (pg1 ++ (compile_aexp (map fst r) e1)) (add :: pg2) (v1 :: stk))
+  as [ec2 Pec2].
 exists (ec1 + ec2 + 1)%nat.
 simpl.
 revert Pec1 Pec2; rewrite <-!app_assoc; simpl.
@@ -213,10 +215,10 @@ set (pg := pg1 ++ _); intros Pec1 Pec2.
 assert 
   (both_exp : exec_asm (ec1 + ec2) pg stk (env_to_mem r) (length pg1) =
     (v2 :: v1 :: stk, env_to_mem r, 
-    (length pg1 + length (compile_aexp r e1) +
-     length (compile_aexp r e2)))%nat).
+    (length pg1 + length (compile_aexp (map fst r) e1) +
+     length (compile_aexp (map fst r) e2)))%nat).
   rewrite (exec_asm_seq pg _ (v1 :: stk) _ (env_to_mem r)
-    _ _ _ (length pg1 + length (compile_aexp r e1))%nat Pec1).
+    _ _ _ (length pg1 + length (compile_aexp (map fst r) e1))%nat Pec1).
   easy.
 rewrite app_length.
 rewrite (exec_asm_seq _ _ (v2 :: v1 :: stk) _ (env_to_mem r)
@@ -232,17 +234,19 @@ Lemma exec_bexp :
   forall env e1 e2 v pg1 pg2 stk,
   beval env (blt e1 e2) v ->
   exists ec, 
-  exec_asm ec (pg1 ++ compile_bexp env (blt e1 e2) ++ pg2)
+  exec_asm ec (pg1 ++ compile_bexp (map fst env) (blt e1 e2) ++ pg2)
        stk (env_to_mem env) (length pg1) =
   (Z.b2z (negb v) :: stk, env_to_mem env, 
-   (length pg1 + length (compile_bexp env (blt e1 e2)))%nat).
+   (length pg1 + length (compile_bexp (map fst env) (blt e1 e2)))%nat).
 Proof.
 intros env e1 e2 v pg1 pg2 stk dyn.
 inversion dyn as [r e1' e2' v1 v2 ev1 ev2 cmp1| 
                   r e1' e2' v1 v2 ev1 ev2 cmp2].
-  destruct (exec_aexp env e1 v1 pg1 (compile_aexp env e2 ++ [cmp] ++ pg2)
+  destruct (exec_aexp env e1 v1 pg1 (compile_aexp
+                                            (map fst env) e2 ++ [cmp] ++ pg2)
                     stk ev1) as [ec1 Pec1].
-  destruct (exec_aexp env e2 v2 (pg1 ++ compile_aexp env e1) ([cmp] ++ pg2)
+  destruct (exec_aexp env e2 v2 (pg1 ++ compile_aexp
+                                       (map fst env) e1) ([cmp] ++ pg2)
               (v1 :: stk) ev2) as [ec2 Pec2].
   revert Pec1 Pec2; simpl; rewrite <-!app_assoc; simpl; set (pg := pg1 ++ _).
   rewrite app_length.
@@ -250,10 +254,11 @@ inversion dyn as [r e1' e2' v1 v2 ev1 ev2 cmp1|
   assert 
     (both_exp : exec_asm (ec1 + ec2) pg stk (env_to_mem env) (length pg1) =
     (v2 :: v1 :: stk, env_to_mem env, 
-    (length pg1 + length (compile_aexp env e1) +
-     length (compile_aexp env e2)))%nat).
+    (length pg1 + length (compile_aexp (map fst env) e1) +
+     length (compile_aexp (map fst env) e2)))%nat).
     rewrite (exec_asm_seq pg _ (v1 :: stk) _ (env_to_mem env)
-      _ _ _ (length pg1 + length (compile_aexp env e1))%nat Pec1).
+      _ _ _ (length pg1 +
+              length (compile_aexp (map fst env) e1))%nat Pec1).
     easy.
   rewrite (exec_asm_seq _ _ (v2 :: v1 :: stk) _ (env_to_mem env)
             _ _ _ _ both_exp).
@@ -264,9 +269,11 @@ inversion dyn as [r e1' e2' v1 v2 ev1 ev2 cmp1|
   assert (cmpv : v2 <=? v1 = false) by now rewrite Z.leb_gt.
   now rewrite cmpv, !Nat.add_assoc.
 
-destruct (exec_aexp env e1 v1 pg1 (compile_aexp env e2 ++ [cmp] ++ pg2)
+destruct (exec_aexp env e1 v1 pg1
+             (compile_aexp (map fst env) e2 ++ [cmp] ++ pg2)
                     stk ev1) as [ec1 Pec1].
-destruct (exec_aexp env e2 v2 (pg1 ++ compile_aexp env e1) ([cmp] ++ pg2)
+destruct (exec_aexp env e2 v2 (pg1 ++
+             compile_aexp (map fst env) e1) ([cmp] ++ pg2)
               (v1 :: stk) ev2) as [ec2 Pec2].
 revert Pec1 Pec2; simpl; rewrite <-!app_assoc; simpl; set (pg := pg1 ++ _).
 rewrite app_length.
@@ -274,10 +281,11 @@ intros Pec1 Pec2; exists (ec1 + ec2 + 1)%nat.
 assert 
     (both_exp : exec_asm (ec1 + ec2) pg stk (env_to_mem env) (length pg1) =
     (v2 :: v1 :: stk, env_to_mem env, 
-    (length pg1 + length (compile_aexp env e1) +
-     length (compile_aexp env e2)))%nat).
+    (length pg1 + length (compile_aexp (map fst env) e1) +
+     length (compile_aexp (map fst env) e2)))%nat).
   rewrite (exec_asm_seq pg _ (v1 :: stk) _ (env_to_mem env)
-      _ _ _ (length pg1 + length (compile_aexp env e1))%nat Pec1).
+      _ _ _ (length pg1 +
+             length (compile_aexp (map fst env) e1))%nat Pec1).
   easy.
 rewrite (exec_asm_seq _ _ (v2 :: v1 :: stk) _ (env_to_mem env)
             _ _ _ _ both_exp).
@@ -291,7 +299,8 @@ Qed.
 
 Lemma update_set_nth : forall r x v r', 
   s_update r x v r' ->
-  set_nth (env_to_mem r) (symbol_index r x) v = (env_to_mem r').
+  set_nth (env_to_mem r)
+             (symbol_index (map fst r) x) v = (env_to_mem r').
 Proof.
 induction 1 as [env x v v' | env env' x y v v' upd Ih xny].
   simpl.
@@ -301,78 +310,33 @@ destruct (S.string_dec x y) as [abs | _];[ now case xny |].
 now rewrite Ih.
 Qed.
 
-Lemma update_index r x v r' z :
-  s_update r x v r' ->
-  symbol_index r z = symbol_index r' z.
+Lemma update_index r x v r' :
+  s_update r x v r' -> map fst r = map fst r'.
 Proof.
 induction 1 as [r x v v' | r r' x y v v' up Ih xny].
   easy.
 now simpl; rewrite Ih.
 Qed.
 
-Lemma update_compile_aexp r x v r' e :
-  s_update r x v r' ->
-  compile_aexp r e = compile_aexp r' e.
+Lemma exec_fst_inv r i1 r' : 
+  exec r i1 r' -> map fst r = map fst r'.
 Proof.
-intros up; induction e as [n | y | e1 Ih1 e2 Ih2].
-    now simpl; rewrite (update_index _ _ _ _ _ up).
-  easy.
-now simpl; rewrite Ih1, Ih2.
-Qed.
-
-Lemma update_compile_bexp r x v r' e :
-  s_update r x v r' ->
-  compile_bexp r e = compile_bexp r' e.
-Proof.
-intros up; induction e as [e1 e2].
-now simpl; rewrite !(update_compile_aexp _ _ _ _ _ up).
-Qed.
-
-Lemma update_compile_instr r x v r' i n :
-  s_update r x v r' ->
-  compile_instr r n i = compile_instr r' n i.
-Proof.
-intros up; revert n; induction i as [y e | i1 Ih1 i2 Ih2| b i Ih| ].
-      now intros n; simpl; rewrite (update_index _ _ _ _ _ up),
-        (update_compile_aexp _ _ _ _ _ up).
-    intros n; simpl.
-    now rewrite Ih1, Ih2.
-  intros n; simpl; rewrite (update_compile_bexp _ _ _ _ _ up).
-  now rewrite Ih.
-easy.
-Qed.
-
-Lemma exec_compile_aexp r i1 r' a :
-  exec r i1 r' -> compile_aexp r a = compile_aexp r' a.
-Proof.
-induction 1 as [ r | r r' s e v ev up| r r' r'' i1_1 i1_2 ex1 Ih1 ex2 Ih2 |
-                     r r' r'' b i ev ex1 Ih1 ex2 Ih2|  ]; try easy.
-    now apply (update_compile_aexp _ _ _ _ _ up).
-  now rewrite <- Ih2.
-now rewrite <- Ih2.
-Qed.
-
-Lemma exec_compile_instr r i1 r' i2 n :
-  exec r i1 r' ->
-  compile_instr r n i2 = compile_instr r' n i2.
-Proof.
-induction 1 as [ r | r r' s e v ev up| r r' r'' i1_1 i1_2 ex1 Ih1 ex2 Ih2 |
-                     r r' r'' b i ev ex1 Ih1 ex2 Ih2|  ].
-        easy.
-      now apply (update_compile_instr _ _ _ _ _ _ up).
-    now rewrite <- Ih2.
-  now rewrite <- Ih2.
-easy.
+induction 1 as [ | r r' x a v ev up |
+   r r' r'' i1 i2 ex1 Ih1 ex2 Ih2 | r r' r'' b i ev ex1 Ih1 ex2 Ih2 | ]; auto.
+- now apply (update_index _ _ _ _ up).
+- now rewrite <- Ih2.
+- now rewrite <- Ih2.
 Qed.
 
 Lemma compile_instr_complete :
   forall env env' i pg1 pg2 stk,
   exec env i env' ->
   exists ec, 
-  exec_asm ec (pg1 ++ compile_instr env (length pg1) i ++ pg2)
+  exec_asm ec
+     (pg1 ++ compile_instr (map fst env) (length pg1) i ++ pg2)
        stk (env_to_mem env) (length pg1) =
   (stk, env_to_mem env', 
-   (length pg1 + length (compile_instr env (length pg1) i))%nat).
+   (length pg1 + length (compile_instr (map fst env) (length pg1) i))%nat).
 Proof.
 intros env env' i pg1 pg2 stk dyn; revert pg1 pg2 stk.
 induction dyn as [ | env env' x e v ev up |
@@ -382,7 +346,8 @@ induction dyn as [ | env env' x e v ev up |
         now exists 0%nat; simpl; rewrite Nat.add_0_r.
       intros pg1 pg2 stk.
       destruct 
-         (exec_aexp env e v pg1 (store (symbol_index env x) :: pg2) stk) as
+         (exec_aexp env e v pg1 
+              (store (symbol_index (map fst env) x) :: pg2) stk) as
         [ec Pec]; auto.
       exists (ec + 1)%nat.
       simpl; rewrite <-!app_assoc; simpl; set (pg := pg1 ++ _).
@@ -396,14 +361,15 @@ induction dyn as [ | env env' x e v ev up |
       now rewrite t2, app_length, Nat.add_0_r, Nat.add_assoc.
     intros pg1 pg2 stk.
     destruct (Ih1 pg1
-               (compile_instr env
-                  (length pg1 + length (compile_instr env (length pg1) i1))
+               (compile_instr (map fst env)
+                  (length pg1 + 
+                   length (compile_instr (map fst env) (length pg1) i1))
                    i2 ++ pg2) stk) as [ec1 Pec1].
     revert Pec1; set (pg := (pg1 ++ _)); intros Pec1.
-    destruct (Ih2 (pg1 ++ (compile_instr env (length pg1) i1)) pg2 stk)
+    destruct (Ih2 (pg1 ++ compile_instr (map fst env) (length pg1) i1) pg2 stk)
         as [ec2 Pec2].
     revert Pec2; rewrite <-!app_assoc, app_length.
-    rewrite <-! (exec_compile_instr _ _ _ _ _ dyn1); fold pg; intros Pec2.
+    rewrite <- (exec_fst_inv  _ _ _ dyn1); fold pg; intros Pec2.
     simpl; rewrite <-!app_assoc, !app_length; fold pg.
     exists (ec1 + ec2)%nat.
     assert (t1 := exec_asm_seq pg _ _ _ _ _ ec2 _ _ Pec1).
@@ -414,20 +380,23 @@ induction dyn as [ | env env' x e v ev up |
   repeat simpl (length [_]).
   set (middle_pc := (_ + 1 + 1)%nat).
   set (last_pc := (_ + 2)%nat).
-  change (branch last_pc :: compile_instr env middle_pc i ++ [goto (length pg1)])
+  change (branch last_pc :: compile_instr (map fst env) middle_pc i
+              ++ [goto (length pg1)])
      with
-   ([branch last_pc] ++ compile_instr env middle_pc i ++ [goto (length pg1)]).
+   ([branch last_pc] ++ compile_instr (map fst env) middle_pc i
+              ++ [goto (length pg1)]).
   rewrite <-!app_assoc.
   set (pg := pg1 ++ _).
   destruct (exec_bexp _ _ _ _ pg1
               ([branch last_pc] ++
-               compile_instr env (length pg1 +
-                 length (compile_bexp env (blt e1 e2)) + 1) i
+               compile_instr (map fst env) (length pg1 +
+                 length (compile_bexp (map fst env) (blt e1 e2)) + 1) i
                 ++ [goto (length pg1)] ++ pg2) stk ev) as [ec1 Pec1].
   revert Pec1; cbn [compile_instr compile_bexp].
   rewrite !app_length, !Nat.add_assoc, <- !app_assoc.
   simpl (length [ _ ]); fold middle_pc; fold pg; intros Pec1.
-  destruct (Ih1 (pg1 ++ compile_bexp env (blt e1 e2) ++ [branch last_pc])
+  destruct (Ih1 (pg1 ++ compile_bexp (map fst env) (blt e1 e2)
+               ++ [branch last_pc])
               ([goto (length pg1)] ++ pg2) stk) as [ec2 Pec2].
   revert Pec2; cbn [compile_instr compile_bexp].
   rewrite !app_length, !Nat.add_assoc, <- !app_assoc.
@@ -437,19 +406,20 @@ induction dyn as [ | env env' x e v ev up |
   revert Pec3; cbn [compile_instr compile_bexp].
   rewrite !app_length, !Nat.add_assoc, <- !app_assoc.
   simpl (length [cmp]); simpl (length [branch _]).
-  rewrite <-! (exec_compile_aexp _ _ _ _ dyn1).
-  rewrite <-! (exec_compile_instr _ _ _ _ _ dyn1).
+  rewrite <- ! (exec_fst_inv _ _ _ dyn1).
   fold middle_pc; fold last_pc.
-  change (branch last_pc :: compile_instr env middle_pc i ++
+  change (branch last_pc :: compile_instr (map fst env) middle_pc i ++
           [goto (length pg1)]) with
-     ([branch last_pc] ++ compile_instr env middle_pc i ++ [goto (length pg1)]).
+     ([branch last_pc] ++ compile_instr (map fst env) middle_pc i ++
+          [goto (length pg1)]).
   rewrite <- !app_assoc; fold pg; intros Pec3.
   exists (ec1 + (1 + (ec2 + (1 + ec3))))%nat.
   rewrite (exec_asm_seq pg _ (Z.b2z (negb true) :: stk) _ _ _ _ _ _ Pec1).
   rewrite (exec_asm_seq pg (Z.b2z (negb true) :: stk) stk (env_to_mem env)
              (env_to_mem env) 1 (ec2 + (1 + ec3))
-             (length pg1 + length (compile_aexp env e1) +
-                  length (compile_aexp env e2) + 1) middle_pc); cycle 1.
+             (length pg1 + length (compile_aexp (map fst env) e1) +
+                  length (compile_aexp (map fst env) e2) + 1) middle_pc);
+         cycle 1.
     simpl; unfold pg; rewrite <-!Nat.add_assoc.
     repeat (rewrite nth_error_app2, minus_plus; [ | lia]).
     now simpl; rewrite !Nat.add_assoc.
@@ -473,15 +443,17 @@ rewrite !app_length, !Nat.add_assoc, <-! app_assoc.
 repeat simpl (length [_]).
 set (middle_pc := (_ + 1 + 1)%nat).
 set (last_pc := (_ + 2)%nat).
-change (branch last_pc :: compile_instr env middle_pc i ++ [goto (length pg1)])
+change (branch last_pc :: compile_instr (map fst env) middle_pc i
+    ++ [goto (length pg1)])
     with
- ([branch last_pc] ++ compile_instr env middle_pc i ++ [goto (length pg1)]).
+ ([branch last_pc] ++ compile_instr (map fst env) middle_pc i
+    ++ [goto (length pg1)]).
 rewrite <-!app_assoc.
 set (pg := pg1 ++ _).
 destruct (exec_bexp _ _ _ _ pg1
             ([branch last_pc] ++
-             compile_instr env (length pg1 +
-               length (compile_bexp env (blt e1 e2)) + 1) i
+             compile_instr (map fst env) (length pg1 +
+               length (compile_bexp (map fst env) (blt e1 e2)) + 1) i
               ++ [goto (length pg1)] ++ pg2) stk ev) as [ec1 Pec1].
 revert Pec1; cbn [compile_instr compile_bexp].
 rewrite !app_length, !Nat.add_assoc, <- !app_assoc.
